Declarative/BasicProperties.v
@@ -1,0 +1,253 @@
+Require Export Declarative.LanguageUtil.
+Require Import Program.Equality.
+
+Import ListNotations.
+
+Theorem weakening : forall Γ1 Γ2 Γ3 e1 e2 A,
+    Γ1 ,, Γ3 ⊢ e1 <: e2 : A ->
+    ⊢ Γ1 ,, Γ2 ,, Γ3 ->
+    Γ1 ,, Γ2 ,, Γ3 ⊢ e1 <: e2 : A.
+Proof.
+  intros until A. intro Hsub.
+  dependent induction Hsub; intro Hwf.
+  - apply s_var.
+    + assumption.
+    + now apply var_in_ctx_weakening.
+  - now apply s_lit.
+  - now apply s_star.
+  - now apply s_int.
+  - apply s_abs with (L `union` dom (Γ1 ,, Γ2 ,, Γ3)).
+    + now apply IHHsub.
+    + intros. distribute_ctx. apply H0.
+      * auto.
+      * reflexivity.
+      * eapply wf_cons.
+        ** exact Hwf.
+        ** auto.
+        ** now apply IHHsub.
+  - apply s_pi with (L `union` dom (Γ1 ,, Γ2 ,, Γ3)) k1.
+    + now apply IHHsub1.
+    + now apply IHHsub2.
+    + now apply IHHsub3.
+    + intros. distribute_ctx. apply H0.
+      * auto.
+      * reflexivity.
+      * eapply wf_cons.
+        ** assumption.
+        ** auto.
+        ** now apply IHHsub1.
+    + intros. distribute_ctx. apply H2.
+      * auto.
+      * reflexivity.
+      * eapply wf_cons.
+        ** assumption.
+        ** auto.
+        ** now apply IHHsub2.
+  - apply s_app with A.
+    + now apply IHHsub1.
+    + now apply IHHsub2.
+  - apply s_forall with (L `union` dom (Γ1 ,, Γ2 ,, Γ3)) k.
+    + now apply IHHsub.
+    + intros. distribute_ctx. apply H0.
+      * auto.
+      * reflexivity.
+      * eapply wf_cons.
+        ** assumption.
+        ** auto.
+        ** now apply IHHsub.
+  - apply s_forall_l with (L `union` dom (Γ1 ,, Γ2 ,, Γ3)) e k.
+    + assumption.
+    + now apply IHHsub1.
+    + now apply IHHsub2.
+    + now apply IHHsub3.
+    + intros. distribute_ctx. apply H1.
+      * auto.
+      * reflexivity.
+      * eapply wf_cons.
+        ** assumption.
+        ** auto.
+        ** now apply IHHsub1.
+  - apply s_forall_r with (L `union` dom (Γ1 ,, Γ2 ,, Γ3)) k.
+    + now apply IHHsub1.
+    + now apply IHHsub2.
+    + intros. distribute_ctx. apply H0.
+      * auto.
+      * reflexivity.
+      * eapply wf_cons.
+        ** assumption.
+        ** auto.
+        ** now apply IHHsub1.
+  - apply s_forall_2 with (L `union` dom (Γ1 ,, Γ2 ,, Γ3)) k.
+    + now apply IHHsub.
+    + intros. distribute_ctx. apply H0.
+      * auto.
+      * reflexivity.
+      * eapply wf_cons.
+        ** assumption.
+        ** auto.
+        ** now apply IHHsub.
+  - apply s_sub with A k.
+    + now apply IHHsub1.
+    + now apply IHHsub2.
+Qed.
+
+Corollary weakening_cons : forall Γ x X e1 e2 A,
+    Γ ⊢ e1 <: e2 : A ->
+    ⊢ Γ , x : X ->
+    Γ , x : X ⊢ e1 <: e2 : A.
+Proof.
+  intros.
+  replace (Γ , x : X) with (Γ ,, (x ~ X) ,, [])  by reflexivity.
+  now apply weakening.
+Qed.
+
+Hint Resolve weakening_cons : core.
+
+Corollary weakening_app : forall Γ Γ' e1 e2 A,
+    Γ ⊢ e1 <: e2 : A ->
+    ⊢ Γ ,, Γ' ->
+    Γ ,, Γ' ⊢ e1 <: e2 : A.
+Proof.
+  intros.
+  replace (Γ ,, Γ') with (Γ ,, Γ' ,, []) by reflexivity.
+  now apply weakening.
+Qed.
+
+Theorem reflexivity_r : forall Γ e1 e2 A, Γ ⊢ e1 <: e2 : A -> Γ ⊢ e2 : A.
+Proof.
+  intros.
+  induction H.
+  - auto.
+  - auto.
+  - auto.
+  - auto.
+  - apply s_abs with L.
+    + assumption.
+    + intros. now apply H1.
+  - apply s_pi with L k1.
+    + assumption.
+    + assumption.
+    + assumption.
+    + auto.
+    + auto.
+  - apply s_app with A.
+    + assumption.
+    + assumption.
+  - apply s_forall with L k.
+    + assumption.
+    + auto.
+  - assumption.
+  - apply s_forall_r with (L `union` dom G `union` (fv_expr (e_all B C))) k.
+    + assumption.
+    + apply s_forall_2 with L k.
+      * assumption.
+      * apply H2.
+    + intros.
+      apply s_forall_l with (add x (L `union` dom G)) (e_var_f x) k.
+      * auto.
+      * eapply weakening_cons; eauto.
+      * eauto.
+      * auto.
+      * intros.
+        replace (G , x : B , x0 : B) with (G ,, x ~ B ,, x0 ~ B) by reflexivity.
+        apply weakening.
+        ** apply H2. auto.
+        ** eapply wf_cons.
+          ++ eapply wf_cons; eauto.
+          ++ eauto.
+          ++ apply weakening_cons; eauto.
+  - apply s_forall_2 with L k.
+    + assumption.
+    + apply H1.
+  - apply s_sub with A k.
+    + assumption.
+    + assumption.
+Qed.
+
+Theorem reflexivity_l : forall Γ e1 e2 A, Γ ⊢ e1 <: e2 : A -> Γ ⊢ e1 : A.
+Proof.
+  intros. induction H.
+  - now apply s_var.
+  - now apply s_lit.
+  - now apply s_star.
+  - now apply s_int.
+  - eapply s_abs.
+    + assumption.
+    + intros x Hxl.
+      apply H1.
+      eassumption.
+  - eapply s_pi; eauto.
+  - now apply s_app with A.
+  - now apply s_forall with L k.
+  - apply s_forall_2 with L k.
+    + assumption.
+    + apply H3.
+  - assumption.
+  - apply s_forall_2 with L k; assumption.
+  - eauto.
+Qed.
+
+Hint Resolve reflexivity_l : core.
+
+Lemma wf_narrowing : forall Γ1 Γ2 x A B,
+    ⊢ Γ1 , x : B ,, Γ2 ->
+    Γ1 ⊢ A <: B : * ->
+    ⊢ Γ1 , x : A ,, Γ2.
+Proof.
+Admitted.
+
+
+Theorem ctx_narrowing : forall Γ1 Γ2 x A B C e1 e2 k,
+  Γ1 , x : B ,, Γ2 ⊢ e1 <: e2 : C ->
+  Γ1 ⊢ A <: B : e_kind k ->
+  Γ1 , x : A ,, Γ2 ⊢ e1 <: e2 : C.
+Proof.
+  intros.
+  remember (Γ1 , x : B ,, Γ2) as Γ.
+  generalize HeqΓ. clear HeqΓ.
+  generalize Γ2. clear Γ2.
+  Check sub_mut.
+  apply sub_mut with
+    (P := fun Γ e1 e2 C (_ : Γ ⊢ e1 <: e2 : C) =>
+        forall Γ2, Γ = Γ1 , x : B ,, Γ2 -> Γ1 , x : A ,, Γ2 ⊢ e1 <: e2 : C)
+    (P0 := fun Γ (_ : ⊢ Γ) =>
+        forall Γ2, Γ = Γ1 , x : B ,, Γ2 -> ⊢ Γ1 , x : A ,, Γ2); intros; subst.
+  - assert ({x = x0} + {x <> x0}) as [E | NE] by apply eq_dec.
+    + subst. apply weakening_app; auto.
+      assert (A0 = B) by now apply binds_type_equal with Γ1 x0 Γ2. subst.
+      apply s_sub with A k.
+      * apply s_var; eauto.
+      * apply weakening_cons; eauto.
+    + apply s_var.
+      * auto.
+      * now apply binds_type_not_equal with B.
+  - auto.
+  - auto.
+  - auto.
+  - eauto.
+  - apply s_pi with (add x L) k1; auto.
+  - eauto.
+  - eauto.
+  - apply s_forall_l with L e k0; eauto 3.
+  - apply s_forall_r with (add x L) k0; auto.
+  - eauto.
+  - eauto.
+
+  (* ⊢ Γ1 , x : B ,, Γ2 → Γ1 ⊢ A <: B : * → ⊢ Γ1 , x : A ,, Γ2 *)
+  - destruct Γ2; inversion H1.
+  - destruct Γ2; try destruct p; inversion H3; subst.
+    + eapply wf_cons; eauto.
+    + eapply wf_cons; auto.
+
+  - assumption.
+Qed.
+
+Corollary ctx_narrowing_cons : forall Γ1 x A B C e1 e2 k,
+    Γ1 , x : A ⊢ e1 <: e2 : C ->
+    Γ1 ⊢ B <: A : e_kind k ->
+    Γ1, x : B ⊢ e1 <: e2 : C.
+Proof.
+  intros.
+  replace (Γ1 , x : B) with (Γ1 ,, x ~ B ,, []) by reflexivity.
+  apply ctx_narrowing with A k; auto.
+Qed.
