Declarative/KindReasoning.v
@@ -1,0 +1,455 @@
+Require Import Declarative.BasicProperties.
+
+Lemma box_never_welltype : forall Γ A,
+    ~ (Γ ⊢ BOX : A).
+Proof.
+  intros. intro.
+  dependent induction H; auto.
+Qed.
+
+Lemma star_type_inversion : forall Γ A,
+    Γ ⊢ * : A -> A = BOX.
+Proof.
+  intros.
+  dependent induction H.
+  - reflexivity.
+  - assert (A = BOX) by auto. subst.
+    apply reflexivity_l in H0. apply box_never_welltype in H0. contradiction.
+Qed.
+
+
+Lemma star_type_inversion_r : forall Γ A B,
+    Γ ⊢ * <: A : B -> B = BOX.
+Proof.
+  intros. apply star_type_inversion with Γ.
+  now apply reflexivity_l with A.
+Qed.
+
+Lemma star_type_inversion_l : forall Γ A B,
+    Γ ⊢ A <: * : B -> B = BOX.
+Proof.
+  intros.
+  apply star_type_inversion with Γ.
+  now apply reflexivity_r with A.
+Qed.
+
+Lemma star_sub_inversion_l : forall Γ A B,
+    Γ ⊢ A <: * : B -> A = *.
+Proof.
+  intros.
+  dependent induction H.
+  - reflexivity.
+  - apply star_type_inversion_l in H2. discriminate.
+  - now apply IHusub1.
+Qed.
+
+Lemma star_sub_inversion_r : forall Γ A B,
+    Γ ⊢ * <: A : B -> A = *.
+Proof.
+  intros.
+  dependent induction H.
+  - reflexivity.
+  - apply star_type_inversion in H0. discriminate.
+  - now apply IHusub1.
+Qed.
+
+Lemma num_not_of_star : forall Γ n,
+    Γ ⊢ e_num n : * -> False.
+Proof.
+  intros. dependent induction H.
+  - assert (e_kind k = BOX).
+    eapply star_type_inversion_l; eauto. inversion H1. subst.
+    apply star_sub_inversion_l in H0.
+    now eapply IHusub1.
+Qed.
+
+Lemma int_of_star : forall Γ A,
+    Γ ⊢ e_int : A -> A = *.
+Proof.
+  intros.
+  dependent induction H.
+  - reflexivity.
+  - assert ( A = * ) by now apply IHusub1. subst.
+    now eapply star_sub_inversion_r in H0.
+Qed.
+
+Lemma abs_not_of_star : forall Γ A B,
+    Γ ⊢ e_abs A B : * -> False.
+Proof.
+  intros.
+  dependent induction H.
+  - apply star_sub_inversion_l in H0.
+    now eapply IHusub1.
+Qed.
+
+Lemma bind_not_of_star : forall Γ A B,
+    Γ ⊢ e_bind A B : * -> False.
+Proof.
+  intros.
+  dependent induction H.
+  - apply star_sub_inversion_l in H0.
+    now eapply IHusub1.
+Qed.
+
+Lemma var_star_inversion : forall Γ x,
+    Γ ⊢ e_var_f x : * -> x : * ∈ Γ.
+Proof.
+  intros.
+  dependent induction H.
+  - assumption.
+  - apply star_sub_inversion_l in H0.
+    now apply IHusub1.
+Qed.
+
+Lemma kind_sub_inversion_l : forall Γ ek kr k,
+    Γ ⊢ ek <: e_kind kr : k -> ek = * /\ kr = k_star /\ k = BOX.
+Proof.
+  intros.
+  dependent induction H.
+  - auto.
+  - edestruct IHusub3. reflexivity. destruct H6. discriminate.
+  - edestruct IHusub1 as [E1 [E2 E3]]; auto.
+    subst.
+    apply reflexivity_l in H0. now apply box_never_welltype in H0.
+Qed.
+
+Inductive head_kind : expr -> kind -> Prop :=
+| h_kind   : forall k, head_kind (e_kind k) k
+| h_pi     : forall A B k,
+    head_kind B k -> head_kind (e_pi A B) k
+| h_forall : forall A B k,
+    head_kind B k -> head_kind (e_all A B) k
+.
+
+Hint Constructors head_kind : core.
+
+Lemma head_kind_invert_subst_rec : forall A e k n,
+    head_kind (open_expr_wrt_expr_rec n e A) k -> head_kind e k \/ head_kind A k.
+Proof.
+  induction A; simpl; intros e k' n' K; try solve [inversion K].
+  - destruct (n' == n); auto.
+  - auto.
+  - inversion K; subst. destruct IHA2 with e k' (S n'); auto.
+  - inversion K; subst. destruct IHA2 with e k' (S n'); auto.
+Qed.
+
+Lemma head_kind_invert_subst : forall A e k,
+    head_kind (A <^^> e) k -> head_kind e k \/ head_kind A k.
+Proof.
+  unfold open_expr_wrt_expr.
+  intros. now apply head_kind_invert_subst_rec with 0.
+Qed.
+
+Lemma head_kind_invert_subst_var : forall A x k,
+    head_kind (A <^> x) k -> head_kind A k.
+Proof.
+  intros.
+  apply head_kind_invert_subst in H as [|].
+  + inversion H.
+  + assumption.
+Qed.
+
+Lemma head_kind_subst_rec : forall A e k n,
+    head_kind A k -> head_kind (open_expr_wrt_expr_rec n e A) k.
+Proof.
+  induction A; simpl; intros e k' n' K; inversion K; eauto.
+Qed.
+
+Lemma head_kind_subst : forall A e k,
+    head_kind A k -> head_kind (A <^^> e) k.
+Proof.
+  intros. now apply head_kind_subst_rec.
+Qed.
+
+Lemma head_kind_subst_var : forall A x k,
+    head_kind A k -> head_kind (A <^> x) k.
+Proof.
+  intros. now apply head_kind_subst_rec.
+Qed.
+
+Hint Resolve head_kind_invert_subst_var : core.
+Hint Resolve head_kind_subst : core.
+Hint Resolve head_kind_invert_subst_var : core.
+
+Lemma head_kind_not_star : forall Γ e k,
+    Γ ⊢ e : * -> head_kind e k -> False.
+Proof.
+  intros. generalize dependent k.
+  dependent induction H; intros k' K; inversion K; subst.
+  - pick fresh x. apply H5 with x k'; eauto.
+  - pick fresh x. apply H4 with x k'; eauto.
+  - now apply IHusub2 with k'.
+  - pick fresh x. apply H1 with x k'; eauto.
+  - apply kind_sub_inversion_l in H0 as [E1 [E2 E3]]. subst.
+    apply kind_sub_inversion_l in H as [E4 [E5 E6]]. subst.
+    inversion E6.
+  - apply kind_sub_inversion_l in H0 as [E1 [E2 E3]]. subst.
+    now apply IHusub1 with k'.
+  - apply kind_sub_inversion_l in H0 as [E1 [E2 E3]]. subst.
+    now apply IHusub1 with k'.
+Qed.
+
+Lemma head_kind_sub_r : forall Γ e1 e2 A,
+    Γ ⊢ e1 <: e2 : A -> forall k, head_kind e1 k -> head_kind e2 k.
+Proof.
+  intros Γ e1 e2 k Hsub.
+  dependent induction Hsub; intros k' K; try solve [inversion K].
+  - assumption.
+  - pick fresh x. inversion K. eauto.
+  - inversion K. subst. assert False.
+    + pick fresh x.
+      eapply head_kind_not_star; eauto.
+    + contradiction.
+  - assert False.
+    + pick fresh x.
+      eapply head_kind_not_star; eauto.
+    + contradiction.
+  - inversion K. subst. assert False.
+    + pick fresh x.
+      eapply head_kind_not_star.
+      eapply reflexivity_r. apply H. auto.
+      eapply H0; eauto.
+    + contradiction.
+  - eauto.
+Qed.
+
+Lemma head_kind_sub_l : forall Γ e1 e2 A,
+    Γ ⊢ e1 <: e2 : A -> forall k, head_kind e2 k -> head_kind e1 k.
+Proof.
+  intros Γ e1 e2 A Hsub.
+  induction Hsub; intros k' K; try solve [inversion K].
+  - assumption.
+  - pick fresh x. inversion K; eauto.
+  - assert False.
+    + eapply head_kind_not_star. eapply reflexivity_l. eauto.
+      eapply IHHsub3. eassumption.
+    + contradiction.
+  - inversion K; subst. assert False.
+    + pick fresh x. eapply head_kind_not_star; eauto.
+    + contradiction.
+  - inversion K; subst. assert False.
+    + pick fresh x. eapply head_kind_not_star. eapply reflexivity_l.
+      all: eauto.
+    + contradiction.
+  - eauto.
+Qed.
+
+Lemma head_kind_var_consistent : forall Γ x A B k,
+    Γ ⊢ e_var_f x : A -> x : B ∈ Γ -> head_kind B k -> head_kind A k.
+Proof.
+  intros until k. intro Hsub.
+  dependent induction Hsub; intros.
+  - assert (A = B) by (eapply binds_consistent; eauto).
+    now rewrite H3.
+  - eapply head_kind_sub_r. apply Hsub2.
+    now eapply IHHsub1.
+Qed.
+
+Lemma head_kind_unique : forall e k1 k2,
+    head_kind e k1 -> head_kind e k2 -> k1 = k2.
+Proof.
+  intros.
+  generalize dependent k2.
+  induction H; intros k2' K; inversion K; subst;
+    pick fresh x; eauto.
+Qed.
+
+Lemma head_kind_star_of_box : forall Γ e A,
+    Γ ⊢ e : A -> head_kind e k_star -> A = BOX.
+Proof.
+  intros Γ e A Hsub Hk. dependent induction Hsub; try solve [inversion Hk].
+  - auto.
+  - inversion Hk; subst.
+    pick fresh x. apply H2 with x; auto.
+  - inversion Hk. subst. pick fresh x. apply H1 with x; auto.
+  - apply IHHsub2; auto.
+  - inversion Hk. subst. pick fresh x. apply H0 with x; auto.
+  - assert (A = BOX) by auto. subst.
+    apply reflexivity_l in Hsub2. now apply box_never_welltype in Hsub2.
+Qed.
+
+Lemma head_kind_box_never_welltype : forall Γ e A,
+    Γ ⊢ e : A -> head_kind e k_box -> False.
+Proof.
+  intros Γ e A Hsub Hk.
+  dependent induction Hsub; inversion Hk; subst;
+    solve [auto | pick_fresh x; eauto ].
+Qed.
+
+Lemma pi_box_never_welltype : forall Γ A B,
+    Γ ⊢ e_pi BOX A : B -> False.
+Proof.
+  intros. dependent induction H.
+  - now apply box_never_welltype in H.
+  - now apply IHusub1 with A.
+Qed.
+
+Lemma bind_type_welltype : forall Γ x A,
+    ⊢ Γ -> x : A ∈ Γ -> exists k, Γ ⊢ A : e_kind k.
+Proof.
+  induction Γ; intros x A Hwf Hsub.
+  - inversion Hsub.
+  - destruct a as [y B]. destruct Hsub; inversion Hwf.
+    + inversion H. subst. eauto.
+    + subst. destruct IHΓ with x A; eauto.
+Qed.
+
+Inductive tail_kind : expr -> kind -> Prop :=
+| tk_pi : forall A k, tail_kind (e_pi (e_kind k) A) k
+| ti_ind : forall A B k, tail_kind B k -> tail_kind (e_pi A B) k
+.
+
+Hint Constructors tail_kind : core.
+
+Lemma tail_kind_subst_rec : forall A e k n,
+    tail_kind A k ->
+    tail_kind (open_expr_wrt_expr_rec n e A) k.
+Proof.
+  induction A; simpl; intros e k' n' Htk; try solve [inversion Htk].
+  - inversion Htk; subst; simpl; auto.
+Qed.
+
+Lemma tail_kind_subst_var : forall A x k,
+    tail_kind A k -> tail_kind (A <^> x) k.
+Proof.
+  intros. now apply tail_kind_subst_rec.
+Qed.
+
+Hint Resolve tail_kind_subst_var : core.
+
+Lemma tail_box_never_welltype : forall Γ e A,
+    Γ ⊢ e : A -> tail_kind e k_box -> False.
+Proof.
+  intros Γ e A Hsub Htk.
+  dependent induction Hsub; try solve [inversion Htk].
+  - inversion Htk; subst.
+    + now apply box_never_welltype in Hsub1.
+    + pick fresh x. apply H2 with x; eauto.
+  - auto.
+Qed.
+
+Lemma open_is_kind_inversion : forall A e k n,
+    e_kind k = open_expr_wrt_expr_rec n e A -> A = e_kind k \/ e = e_kind k.
+Proof.
+  induction A; simpl; intros e k' n' E; try solve [inversion E].
+  - destruct (n' == n); auto.
+  - auto.
+Qed.
+
+Lemma tail_kind_invert_subst_rec : forall A e k n,
+    tail_kind (open_expr_wrt_expr_rec n e A) k ->
+    tail_kind A k \/ tail_kind e k \/ e = e_kind k.
+Proof.
+  induction A; simpl; intros e k' n' Htk; try solve [inversion Htk].
+  - destruct (n' == n); auto.
+  - inversion Htk; subst.
+    + apply open_is_kind_inversion in H0 as [E | E]; subst; auto.
+    + edestruct IHA2 as [H|[H|H]]; eauto.
+Qed.
+
+
+Lemma tail_box_impossible : forall Γ e A,
+    Γ ⊢ e : A -> tail_kind A k_box -> False.
+Proof.
+  intros Γ e A Hsub Htk.
+  dependent induction Hsub; try solve [inversion Htk].
+  - apply bind_type_welltype in H0 as [k Hsub]; auto.
+    eapply tail_box_never_welltype; eauto.
+  - inversion Htk; subst.
+    + now apply box_never_welltype in Hsub.
+    + pick fresh x. eauto.
+  - apply tail_kind_invert_subst_rec in Htk as [Htk | [Htk | E]].
+    + auto.
+    + apply tail_box_never_welltype with G e A; auto.
+    + subst. now apply box_never_welltype in Hsub1.
+  - apply reflexivity_r in Hsub2. eapply tail_box_never_welltype; eauto.
+Qed.
+
+Lemma pi_box_impossible : forall Γ e A,
+    Γ ⊢ e : e_pi BOX A -> False.
+Proof.
+  intros.
+  assert (tail_kind (e_pi BOX A) k_box) by auto.
+  apply tail_box_impossible in H; auto.
+Qed.
+
+Ltac argument_cannot_be_star :=
+  match goal with
+  | H1 : _ ⊢ ?e <: ?e : ?A  |- _ => match goal with
+  | H2 : _ ⊢ _ <: _ : e_pi ?A _ |- _ => match goal with
+  | Hk : head_kind ?e k_star |- _ =>
+    apply head_kind_star_of_box in H1; auto;
+    subst; now apply pi_box_impossible in H2
+  end end end
+.
+
+Ltac argument_cannot_be_kind :=
+  match goal with
+  | H : _ ⊢ ?e <: ?e : ?A  |- _ => match goal with
+  | _ : _ ⊢ _ <: _ : e_pi ?A _ |- _ => match goal with
+  | _ : head_kind ?e ?k |- _ =>
+    destruct k;
+    [> argument_cannot_be_star
+    |  now apply head_kind_box_never_welltype in H
+    ]
+  end end end
+.
+
+Lemma head_kind_consistency : forall Γ e A k1,
+    Γ ⊢ e : A -> head_kind A k1 -> forall B k2, Γ ⊢ e : B -> head_kind B k2 -> k1 = k2.
+Proof.
+  intros until k1. intros Hsub Hk.
+  dependent induction Hsub; intros B' k2' Hsubr Hkr.
+  - dependent induction Hsubr.
+    + assert (A0 = A).
+      * eapply binds_consistent; eauto.
+      * rewrite H3 in Hkr. eapply head_kind_unique; eauto.
+    + assert (head_kind A0 k2').
+      * eapply head_kind_sub_l; eauto.
+      * eauto.
+  - inversion Hk.
+  - inversion Hk. apply star_type_inversion in Hsubr. subst.
+    now inversion Hkr.
+  - apply int_of_star in Hsubr.
+    inversion Hk. subst. now inversion Hkr.
+  - dependent induction Hsubr.
+    + inversion Hk. inversion Hkr. subst. pick fresh x.
+      apply H0 with x (B0 <^> x); eauto 3.
+    + eauto 3 using head_kind_sub_l.
+  - dependent induction Hsubr.
+    + inversion Hk. inversion Hkr. clear H4 H6 IHHsubr1 IHHsubr2 IHHsubr3.
+      subst. pick fresh x.
+      apply H0 with x (e_kind k2'); eauto.
+    + eauto 3 using head_kind_sub_l.
+  - dependent induction Hsubr.
+    + apply head_kind_invert_subst in Hk as [|];
+      apply head_kind_invert_subst in Hkr as [|];
+        try argument_cannot_be_kind.
+      apply IHHsub2 with (e_pi A0 B0); auto.
+    + eauto 3 using head_kind_sub_l.
+  - dependent induction Hsubr.
+    + inversion Hk. inversion Hkr. subst.
+      pick fresh x. apply H0 with x (B0 <^> x); eauto.
+    + eauto 3 using head_kind_sub_l.
+  - dependent induction Hsubr;
+      [> pick_fresh x; apply H1 with x *; eauto 2 ..
+      |  eauto 3 using head_kind_sub_l
+      ].
+  - eauto.
+  - dependent induction Hsubr;
+      [> pick_fresh x; apply H0 with x *; eauto 2 ..
+      | eauto 3 using head_kind_sub_l
+      ].
+  - eauto 3 using head_kind_sub_l.
+Qed.
+
+Lemma kind_consistency : forall Γ e k1 k2,
+    Γ ⊢ e : e_kind k1 -> Γ ⊢ e : e_kind k2 -> k1 = k2.
+Proof.
+  intros.
+  eapply head_kind_consistency.
+  + exact H.
+  + auto.
+  + exact H0.
+  + auto.
+Qed.
