Declarative/Properties.v
@@ -1,346 +1,89 @@
-Require Import Declarative.LanguageUtil.
-Require Import Program.Equality.
-Import ListNotations.
+Require Import Declarative.BasicProperties.
+Require Import Declarative.KindReasoning.
 
-Theorem weakening : forall Γ1 Γ2 Γ3 e1 e2 A,
-    Γ1 ,, Γ3 ⊢ e1 <: e2 : A ->
-    ⊢ Γ1 ,, Γ2 ,, Γ3 ->
-    Γ1 ,, Γ2 ,, Γ3 ⊢ e1 <: e2 : A.
+Theorem transitivity : forall e2 Γ e1 e3 A B,
+  Γ ⊢ e1 <: e2 : A -> Γ ⊢ e2 <: e3 : B -> Γ ⊢ e1 <: e3 : A.
 Proof.
-  intros until A. intro Hsub.
-  dependent induction Hsub; intro Hwf.
-  - apply s_var.
-    + assumption.
-    + now apply var_in_ctx_weakening.
-  - now apply s_lit.
-  - now apply s_star.
-  - now apply s_int.
-  - apply s_abs with (L `union` dom (Γ1 ,, Γ2 ,, Γ3)).
-    + now apply IHHsub.
-    + intros. distribute_ctx. apply H0.
+  intro. assert (lc_expr e2) by admit.
+  induction H; intros Γ e1' e3' A' B' Hsubl;
+    generalize dependent e3'; generalize dependent B'.
+  - dependent induction Hsubl; intros B' e3' Hsubr.
+    + dependent induction Hsubr.
       * auto.
-      * reflexivity.
-      * apply wf_cons.
-        ** exact Hwf.
-        ** auto.
-        ** now apply IHHsub.
-  - apply s_pi with (L `union` dom (Γ1 ,, Γ2 ,, Γ3)).
-    + now apply IHHsub1.
-    + now apply IHHsub2.
-    + now apply IHHsub3.
-    + intros. distribute_ctx. apply H0.
+      * assert ( binds x * G ) by now apply var_star_inversion.
+        apply binds_inversion in H0.
+        destruct H0 as [Γ1 [Γ2 E]].
+        rewrite E in H3, H.
+        assert ( * = A ) by (eapply binds_type_equal; eassumption).
+        rewrite <- H0 in *. apply s_forall_r with L k; eauto.
+      * eauto 3.
+    + eauto.
+    + eauto.
+  - dependent induction Hsubl; intros B' e3' Hsubr.
+    + dependent induction Hsubr.
       * auto.
-      * reflexivity.
-      * apply wf_cons.
-        ** assumption.
-        ** auto.
-        ** now apply IHHsub1.
-    + intros. distribute_ctx. apply H2.
-      * auto.
-      * reflexivity.
-      * apply wf_cons.
-        ** assumption.
-        ** auto.
-        ** now apply IHHsub2.
-  - apply s_app with A.
-    + now apply IHHsub1.
-    + now apply IHHsub2.
-  - apply s_forall with (L `union` dom (Γ1 ,, Γ2 ,, Γ3)).
-    + assumption.
-    + now apply IHHsub.
-    + intros. distribute_ctx. apply H1.
-      * auto.
-      * reflexivity.
-      * apply wf_cons.
-        ** assumption.
-        ** auto.
-        ** now apply IHHsub.
-  - apply s_forall_l with (L `union` dom (Γ1 ,, Γ2 ,, Γ3)) e.
-    + assumption.
-    + assumption.
-    + now apply IHHsub1.
-    + now apply IHHsub2.
-    + now apply IHHsub3.
-    + intros. distribute_ctx. apply H2.
-      * auto.
-      * reflexivity.
-      * apply wf_cons.
-        ** assumption.
-        ** auto.
-        ** now apply IHHsub1.
-  - apply s_forall_r with (L `union` dom (Γ1 ,, Γ2 ,, Γ3)).
-    + assumption.
-    + now apply IHHsub1.
-    + now apply IHHsub2.
-    + intros. distribute_ctx. apply H1.
-      * auto.
-      * reflexivity.
-      * apply wf_cons.
-        ** assumption.
-        ** auto.
-        ** now apply IHHsub1.
-  - apply s_forall_2 with (L `union` dom (Γ1 ,, Γ2 ,, Γ3)).
-    + assumption.
-    + now apply IHHsub.
-    + intros. distribute_ctx. apply H1.
-      * auto.
-      * reflexivity.
-      * apply wf_cons.
-        ** assumption.
-        ** auto.
-        ** now apply IHHsub.
-  - apply s_sub with A.
-    + now apply IHHsub1.
-    + now apply IHHsub2.
-Qed.
-
-Corollary weakening_cons : forall Γ x X e1 e2 A,
-    Γ ⊢ e1 <: e2 : A ->
-    ⊢ Γ , x : X ->
-    Γ , x : X ⊢ e1 <: e2 : A.
-Proof.
-  intros.
-  replace (Γ , x : X) with (Γ ,, (x ~ X) ,, [])  by reflexivity.
-  now apply weakening.
-Qed.
-
-Hint Resolve weakening_cons : core.
-
-Corollary weakening_app : forall Γ Γ' e1 e2 A,
-    Γ ⊢ e1 <: e2 : A ->
-    ⊢ Γ ,, Γ' ->
-    Γ ,, Γ' ⊢ e1 <: e2 : A.
-Proof.
-  intros.
-  replace (Γ ,, Γ') with (Γ ,, Γ' ,, []) by reflexivity.
-  now apply weakening.
-Qed.
-
-Theorem reflexivity_r : forall Γ e1 e2 A, Γ ⊢ e1 <: e2 : A -> Γ ⊢ e2 : A.
-Proof.
-  intros.
-  induction H.
-  - auto.
-  - auto.
-  - auto.
-  - auto.
-  - apply s_abs with L.
-    + assumption.
-    + intros. now apply H1.
-  - apply s_pi with L.
-    + assumption.
-    + assumption.
-    + assumption.
-    + auto.
-    + auto.
-  - apply s_app with A.
-    + assumption.
-    + assumption.
-  - apply s_forall with L.
-    + assumption.
-    + assumption.
-    + auto.
-  - assumption.
-  - apply s_forall_r with (L `union` dom G `union` (fv_expr (e_all B C))).
-    + assumption.
-    + assumption.
-    + apply s_forall_2 with L.
-      * assumption.
-      * assumption.
-      * apply H3.
-    + intros.
-      apply s_forall_l with (add x (L `union` dom G)) (e_var_f x).
-      * auto.
-      * assumption.
-      * apply weakening_cons; auto.
-      * auto.
-      * auto.
-      * intros.
-        replace (G , x : B , x0 : B) with (G ,, x ~ B ,, x0 ~ B) by reflexivity.
-        apply weakening.
-        ** apply H3. auto.
-        ** apply wf_cons.
-          ++ apply wf_cons; auto.
-          ++ auto.
-          ++ apply weakening_cons; auto.
-  - apply s_forall_2 with L.
-    + assumption.
-    + assumption.
-    + apply H2.
-  - apply s_sub with A.
-    + assumption.
-    + assumption.
-Qed.
-(*
-Theorem wf_strengthening : forall Γ1 Γ2 x A,
-    ⊢ Γ1 , x : A ,, Γ2 ->
-    context_fresh x Γ2 ->
-    ⊢ Γ1 ,, Γ2.
-Proof.
+      * apply star_type_inversion in Hsubr2. inversion Hsubr2.
+      * apply IHHsubr1; auto.
+    + eauto.
+    + eauto.
+  - dependent induction Hsubl; intros B' e3' Hsubr.
+    + dependent induction Hsubr.
+      * eauto 3.
+      * apply num_not_of_star in Hsubr2. contradiction.
+      * eauto 3.
+    + eauto 3.
+    + eauto 3.
+  - dependent induction Hsubl; intros B' e3' Hsubr.
+    + dependent induction Hsubr; eauto 3.
+    + eauto 3.
+    + eauto 3.
+  - dependent induction Hsubl; intros B' e3' Hsubr.
+    + dependent induction Hsubr.
+      * eauto 3.
+      * admit.
+      * eauto 3.
+    + eauto 3.
+    + eauto 3.
+  - dependent induction Hsubl; intros B' e3' Hsubr.
+    + dependent induction Hsubr.
+      * apply s_abs with (L `union` L1 `union` L0); eauto 1.
+        intros. apply H1 with x (B0 <^> x); auto 2.
+      * apply abs_not_of_star in Hsubr2. contradiction.
+      * eauto 2.
+    + eauto 3.
+    + eauto 3.
+  - dependent induction Hsubl; intros B' e3' Hsubr.
+    + dependent induction Hsubr.
+      * apply s_pi with (L `union` L0 `union` L1) k3; admit.
+      * admit.
+      * eauto 2.
+    + eauto 3.
+    + eauto 3.
+  - dependent induction Hsubl; intros B' e3' Hsubr.
+    + eauto 3.
+    + admit.
+    + admit.
+    + eauto 3.
+  - dependent induction Hsubl; intros B' e3' Hsubr.
+    + dependent induction Hsubr.
+      * apply s_forall with (L `union` L0 `union` L1) k; eauto 3.
+        intros. eapply H1. eauto. auto. apply H5. auto.
+      * apply bind_not_of_star in Hsubr2. contradiction.
+      * eauto 2.
+    + eauto 3.
+    + eauto 3.
 Admitted.
 
-Lemma var_in_ctx_strengthening : forall Γ1 Γ2 x y (A B : expr),
-    x : A ∈ Γ1 , y : B ,, Γ2 ->
-    y <> x ->
-    x : A ∈ Γ1 ,, Γ2.
-Proof.
-  intros Γ1 Γ2. generalize dependent Γ1.
-  induction Γ2; intros.
-  - destruct H.
-    + inversion H. contradiction.
-    + assumption.
-  - destruct a. destruct H.
-    + inversion H. subst. auto.
-    + unfold binds, In. right.
-      now apply IHΓ2 with y B.
-Qed.
-
-Theorem ctx_strengthening : forall Γ1 Γ2 x A e1 e2 B,
-    Γ1 , x : A ,, Γ2 ⊢ e1 <: e2 : B ->
-    context_fresh x Γ2 ->
-    x # e1 -> x # e2 -> x # B ->
-    Γ1 ,, Γ2 ⊢ e1 <: e2 : B.
-Proof.
-  intros until B. intros Hsub.
-  remember (Γ1 , x : A ,, Γ2) as Γ eqn: Heq.
-  generalize dependent Γ2.
-  generalize dependent A.
-  generalize dependent x.
-  generalize dependent Γ1.
-  apply sub_mut with
-      (P := fun (Γ : context) (e1 e2 B : expr) (Hsub : Γ ⊢ e1 <: e2 : B) =>
-              forall Γ1 x A Γ2, Γ = Γ1 , x : A ,, Γ2 -> context_fresh x Γ2 ->
-w                 x # e1 -> x # e2 -> x # B -> Γ1 ,, Γ2 ⊢ e1 <: e2 : B)
-      (P0 := fun (Γ : context) (Hwf : ⊢ Γ) =>
-               forall Γ1 Γ2 x A, Γ = Γ1 , x : A ,, Γ2 -> context_fresh x Γ2 ->
-                 ⊢ Γ1 ,, Γ2).
-  all: intros; subst; simpl in *.
-  - apply s_var. now apply H with x0 A0.
-    apply var_in_ctx_strengthening with x0 A0; auto 2.
-  - apply s_lit . eauto.
-  - apply s_star. eauto.
-  - apply s_int . eauto.
-  - apply s_abs with (add x (fv_expr A0 `union` L)).
-    + eapply H; eauto.
-    + intros. distribute_ctx.
-      apply H0 with x A0; auto 3.
-  - apply s_pi with (add x (fv_expr A `union` L)).
-    + eapply H ; eauto.
-    + eapply H0; eauto.
-    + eapply H1; eauto.
-    + intros. distribute_ctx.
-      apply H2 with x A; auto 3.
-    + intros. distribute_ctx.
-      apply H3 with x A; auto 3.
-  - admit. (* s_app *)
-  - apply s_forall with (add x (fv_expr A0 `union` L)).
-    + assumption.
-    + eapply H; eauto.
-    + intros. distribute_ctx.
-      apply H0 with x A0; eauto.
-  - admit. (* s_forall_l *)
-  - apply s_forall_r with (add x (fv_expr A0 `union` L)).
-    + assumption.
-    + eapply H; eauto.
-    + intros. distribute_ctx.
-      apply H0 with x A0; auto 3.
-    + auto.
-  - admit. (* s_sub *)
-
-  (* ⊢ Γ1 , x : A ,, Γ2 → context_fresh x Γ2 → ⊢ Γ1 ,, Γ2 *)
-  - destruct Γ2; inversion H.
-  - destruct Γ2.
-    + inversion H1. now subst.
-    + destruct p. inversion H1. subst; simpl in H2; destruct H2.
-      apply wf_cons.
-      * eapply H; eauto.
-      * auto.
-      * eapply H0; eauto.
-  - assumption.
-Admitted.
-*)
-Theorem reflexivity_l : forall Γ e1 e2 A, Γ ⊢ e1 <: e2 : A -> Γ ⊢ e1 : A.
-Proof.
-  intros. induction H.
-  - now apply s_var.
-  - now apply s_lit.
-  - now apply s_star.
-  - now apply s_int.
-  - eapply s_abs.
-    + assumption.
-    + intros x Hxl.
-      apply H1.
-      eassumption.
-  - eapply s_pi; auto.
-  - now apply s_app with A.
-  - now apply s_forall with L.
-  - apply s_forall_2 with L.
-    + assumption.
-    + assumption.
-    + apply H4.
-  - assumption.
-  - apply s_forall_2 with L; assumption.
-  - eauto.
-Qed.
-
-Hint Resolve reflexivity_l : core.
-
-Lemma wf_narrowing : forall Γ1 Γ2 x A B,
-    ⊢ Γ1 , x : B ,, Γ2 ->
-    Γ1 ⊢ A <: B : * ->
-    ⊢ Γ1 , x : A ,, Γ2.
-Proof.
-Admitted.
-
-
-Theorem ctx_narrowing : forall Γ1 Γ2 x A B C e1 e2,
-  Γ1 , x : B ,, Γ2 ⊢ e1 <: e2 : C ->
-  Γ1 ⊢ A <: B : * ->
-  Γ1 , x : A ,, Γ2 ⊢ e1 <: e2 : C.
-Proof.
-  intros.
-  remember (Γ1 , x : B ,, Γ2) as Γ.
-  generalize HeqΓ. clear HeqΓ.
-  generalize Γ2. clear Γ2.
-  Check sub_mut.
-  apply sub_mut with
-    (P := fun Γ e1 e2 C (_ : Γ ⊢ e1 <: e2 : C) =>
-        forall Γ2, Γ = Γ1 , x : B ,, Γ2 -> Γ1 , x : A ,, Γ2 ⊢ e1 <: e2 : C)
-    (P0 := fun Γ (_ : ⊢ Γ) =>
-        forall Γ2, Γ = Γ1 , x : B ,, Γ2 -> ⊢ Γ1 , x : A ,, Γ2); intros; subst.
-  - assert ({x = x0} + {x <> x0}) as [E | NE] by apply eq_dec.
-    + subst. apply weakening_app; auto.
-      assert (A0 = B) by now apply binds_type_equal with Γ1 x0 Γ2. subst.
-      apply s_sub with A.
-      * apply s_var; eauto.
-      * apply weakening_cons; eauto.
-    + apply s_var.
-      * auto.
-      * now apply binds_type_not_equal with B.
-  - auto.
-  - auto.
-  - auto.
-  - eauto.
-  - apply s_pi with (add x L); auto.
-  - eauto.
-  - eauto.
-  - apply s_forall_l with L e; auto.
-  - apply s_forall_r with (add x L); auto.
-  - eauto.
-  - eauto.
-
-  (* ⊢ Γ1 , x : B ,, Γ2 → Γ1 ⊢ A <: B : * → ⊢ Γ1 , x : A ,, Γ2 *)
-  - destruct Γ2; inversion H1.
-  - destruct Γ2; try destruct p; inversion H3; subst.
-    + apply wf_cons; eauto.
-    + apply wf_cons; auto.
-
-  - assumption.
-Qed.
-
-Theorem transitivity : forall Γ e1 e2 e3 A,
+Theorem transitivity' : forall e2 Γ e1 e3 A,
   Γ ⊢ e1 <: e2 : A -> Γ ⊢ e2 <: e3 : A -> Γ ⊢ e1 <: e3 : A.
 Proof.
+  intro. assert (lc_expr e2) by admit.
+  induction H; intros Γ e1' e3' A' Hsubl;
+    generalize dependent e3'.
+  - dependent induction Hsubl; intros e3' Hsubr.
+    + assumption.
+    + eauto.
+    + admit.
 Admitted.
 
 Lemma binds_var_consistent : forall Γ x A B,
@@ -362,15 +105,6 @@ Proof.
         ** apply weakening_cons; auto.
   - admit. (* need transitivity *)
 Admitted.
-
-Theorem num_of_type_int : forall Γ n A,
-    Γ ⊢ e_num n <: e_num n : A -> int_like A.
-Proof.
-  intros.
-  dependent induction H.
-  - constructor.
-  - assert (int_like A) by now apply IHusub1 with n.
-    induction H1. admit.
 
 Theorem type_consistency : forall Γ e1 e2 A B,
   Γ ⊢ e1 : A -> Γ ⊢ e1 <: e2 : B -> Γ ⊢ e1 <: e2 : A.
